\documentclass[fleqn]{article}
\usepackage{fullpage,latexsym}
\newenvironment{VampireProof}{%
   \section{Proof}}{}
\newenvironment{VampireInference}{%
   \begin{array}{c}}{\end{array}}
\newenvironment{VampireInferencePremises}{}{}
\newenvironment{VampirePremise}%
   {\begin{array}{l}}%
   {\end{array}}
\newenvironment{VampireConclusion}%
   {\begin{array}{l}}%
   {\end{array}}
\newcommand{\VampireUnit}[3]{%
   #1.~#2~[#3]}
\newcommand{\VPremiseSeparator}{\\}
\newcommand{\VConclusionSeparator}{\\ \hline}
\newcommand{\Vor}{\vee}
\newcommand{\Vand}{\wedge}
\newcommand{\Vimp}{\rightarrow}
\newcommand{\Viff}{\leftrightarrow}
\newcommand{\Vxor}{\not\Viff}
\newcommand{\VEmptyClause}{\Box}
\begin{document}
\begin{VampireProof}
[$882,29\rightarrow 1056$, resolution]\\*[-2ex]
\[\begin{VampireInference}
\begin{VampirePremise}%
~~\mathit{p} (x_{0},\sigma_{0}(x_{0}))
\end{VampirePremise}
\VPremiseSeparator
\begin{VampirePremise}%
~~\neg \mathit{p} (\sigma_{3}(a0),x_{1})
\end{VampirePremise}
\VConclusionSeparator
\begin{VampireConclusion}
~~\VEmptyClause
\end{VampireConclusion}
\end{VampireInference}
\]
[$20\rightarrow 29$, cnf transformation]\\*[-2ex]
\[\begin{VampireInference}
\begin{VampirePremise}%
~~(\forall x_{1} )\neg \mathit{p} (\sigma_{3}(a0),x_{1})
\end{VampirePremise}
\VConclusionSeparator
\begin{VampireConclusion}
~~\neg \mathit{p} (\sigma_{3}(a0),x_{1})
\end{VampireConclusion}
\end{VampireInference}
\]
[$669,32\rightarrow 882$, resolution]\\*[-2ex]
\[\begin{VampireInference}
\begin{VampirePremise}%
~~\neg \mathit{p} (\mathit{z},x_{1}) \Vor \mathit{p} (x_{0},\sigma_{0}(x_{0}))
\end{VampirePremise}
\VPremiseSeparator
\begin{VampirePremise}%
~~\mathit{p} (\mathit{z},\mathit{z})
\end{VampirePremise}
\VConclusionSeparator
\begin{VampireConclusion}
~~\mathit{p} (x_{0},\sigma_{0}(x_{0}))
\end{VampireConclusion}
\end{VampireInference}
\]
[$31,21\rightarrow 32$, superposition]\\*[-2ex]
\[\begin{VampireInference}
\begin{VampirePremise}%
~~\mathit{p} (\mathit{add} (x_{1},x_{1}),x_{1})
\end{VampirePremise}
\VPremiseSeparator
\begin{VampirePremise}%
~~\mathit{add} (\mathit{z},x_{0}) = x_{0}
\end{VampirePremise}
\VConclusionSeparator
\begin{VampireConclusion}
~~\mathit{p} (\mathit{z},\mathit{z})
\end{VampireConclusion}
\end{VampireInference}
\]
[$1\rightarrow 21$, cnf transformation]\\*[-2ex]
\[\begin{VampireInference}
\begin{VampirePremise}%
~~(\forall x_{0} )\mathit{add} (\mathit{z},x_{0}) = x_{0}
\end{VampirePremise}
\VConclusionSeparator
\begin{VampireConclusion}
~~\mathit{add} (\mathit{z},x_{0}) = x_{0}
\end{VampireConclusion}
\end{VampireInference}
\]
[$25\rightarrow 31$, equality resolution]\\*[-2ex]
\[\begin{VampireInference}
\begin{VampirePremise}%
~~\mathit{p} (x_{0},x_{1}) \Vor \mathit{add} (x_{1},x_{1}) \neq x_{0}
\end{VampirePremise}
\VConclusionSeparator
\begin{VampireConclusion}
~~\mathit{p} (\mathit{add} (x_{1},x_{1}),x_{1})
\end{VampireConclusion}
\end{VampireInference}
\]
[$13\rightarrow 25$, cnf transformation]\\*[-2ex]
\[\begin{VampireInference}
\begin{VampirePremise}%
~~(\forall x_{0} \forall x_{1} )((\neg \mathit{p} (x_{0},x_{1}) \Vor \mathit{add} (x_{1},x_{1}) = x_{0} \Vor \mathit{s} (\mathit{add} (x_{1},x_{1})) = x_{0}) \Vand ((\mathit{add} (x_{1},x_{1}) \neq x_{0} \Vand \mathit{s} (\mathit{add} (x_{1},x_{1})) \neq x_{0}) \Vor \mathit{p} (x_{0},x_{1})))
\end{VampirePremise}
\VConclusionSeparator
\begin{VampireConclusion}
~~\mathit{p} (x_{0},x_{1}) \Vor \mathit{add} (x_{1},x_{1}) \neq x_{0}
\end{VampireConclusion}
\end{VampireInference}
\]
[$584,28\rightarrow 669$, resolution]\\*[-2ex]
\[\begin{VampireInference}
\begin{VampirePremise}%
~~\mathit{p} (\mathit{s} (\sigma_{1}(a0)),\sigma_{2}(a0))
\end{VampirePremise}
\VPremiseSeparator
\begin{VampirePremise}%
~~\neg \mathit{p} (\mathit{s} (\sigma_{1}(a0)),x_{3}) \Vor \mathit{p} (x_{0},\sigma_{0}(x_{0})) \Vor \neg \mathit{p} (\mathit{z},x_{5})
\end{VampirePremise}
\VConclusionSeparator
\begin{VampireConclusion}
~~\neg \mathit{p} (\mathit{z},x_{1}) \Vor \mathit{p} (x_{0},\sigma_{0}(x_{0}))
\end{VampireConclusion}
\end{VampireInference}
\]
[$18\rightarrow 28$, cnf transformation]\\*[-2ex]
\[\begin{VampireInference}
\begin{VampirePremise}%
~~(\forall x_{5} )\neg \mathit{p} (\mathit{z},x_{5}) \Vor (\mathit{p} (\sigma_{1}(a0),\sigma_{2}(a0)) \Vand (\forall x_{3} )\neg \mathit{p} (\mathit{s} (\sigma_{1}(a0)),x_{3})) \Vor (\forall x_{0} )\mathit{p} (x_{0},\sigma_{0}(x_{0}))
\end{VampirePremise}
\VConclusionSeparator
\begin{VampireConclusion}
~~\neg \mathit{p} (\mathit{s} (\sigma_{1}(a0)),x_{3}) \Vor \mathit{p} (x_{0},\sigma_{0}(x_{0})) \Vor \neg \mathit{p} (\mathit{z},x_{5})
\end{VampireConclusion}
\end{VampireInference}
\]
[$30,515\rightarrow 584$, superposition]\\*[-2ex]
\[\begin{VampireInference}
\begin{VampirePremise}%
~~\mathit{p} (\mathit{s} (\mathit{add} (x_{1},x_{1})),x_{1})
\end{VampirePremise}
\VPremiseSeparator
\begin{VampirePremise}%
~~\sigma_{1}(a0) = \mathit{add} (\sigma_{2}(a0),\sigma_{2}(a0))
\end{VampirePremise}
\VConclusionSeparator
\begin{VampireConclusion}
~~\mathit{p} (\mathit{s} (\sigma_{1}(a0)),\sigma_{2}(a0))
\end{VampireConclusion}
\end{VampireInference}
\]
[$454,29\rightarrow 515$, resolution]\\*[-2ex]
\[\begin{VampireInference}
\begin{VampirePremise}%
~~\mathit{p} (x_{0},\sigma_{0}(x_{0})) \Vor \sigma_{1}(a0) = \mathit{add} (\sigma_{2}(a0),\sigma_{2}(a0))
\end{VampirePremise}
\VPremiseSeparator
\begin{VampirePremise}%
~~\neg \mathit{p} (\sigma_{3}(a0),x_{1})
\end{VampirePremise}
\VConclusionSeparator
\begin{VampireConclusion}
~~\sigma_{1}(a0) = \mathit{add} (\sigma_{2}(a0),\sigma_{2}(a0))
\end{VampireConclusion}
\end{VampireInference}
\]
[$221,32\rightarrow 454$, resolution]\\*[-2ex]
\[\begin{VampireInference}
\begin{VampirePremise}%
~~\neg \mathit{p} (\mathit{z},x_{1}) \Vor \mathit{p} (x_{0},\sigma_{0}(x_{0})) \Vor \sigma_{1}(a0) = \mathit{add} (\sigma_{2}(a0),\sigma_{2}(a0))
\end{VampirePremise}
\VPremiseSeparator
\begin{VampirePremise}%
~~\mathit{p} (\mathit{z},\mathit{z})
\end{VampirePremise}
\VConclusionSeparator
\begin{VampireConclusion}
~~\mathit{p} (x_{0},\sigma_{0}(x_{0})) \Vor \sigma_{1}(a0) = \mathit{add} (\sigma_{2}(a0),\sigma_{2}(a0))
\end{VampireConclusion}
\end{VampireInference}
\]
[$158,28\rightarrow 221$, resolution]\\*[-2ex]
\[\begin{VampireInference}
\begin{VampirePremise}%
~~\mathit{p} (\mathit{s} (\sigma_{1}(a0)),\mathit{s} (\sigma_{2}(a0))) \Vor \sigma_{1}(a0) = \mathit{add} (\sigma_{2}(a0),\sigma_{2}(a0))
\end{VampirePremise}
\VPremiseSeparator
\begin{VampirePremise}%
~~\neg \mathit{p} (\mathit{s} (\sigma_{1}(a0)),x_{3}) \Vor \mathit{p} (x_{0},\sigma_{0}(x_{0})) \Vor \neg \mathit{p} (\mathit{z},x_{5})
\end{VampirePremise}
\VConclusionSeparator
\begin{VampireConclusion}
~~\neg \mathit{p} (\mathit{z},x_{1}) \Vor \mathit{p} (x_{0},\sigma_{0}(x_{0})) \Vor \sigma_{1}(a0) = \mathit{add} (\sigma_{2}(a0),\sigma_{2}(a0))
\end{VampireConclusion}
\end{VampireInference}
\]
[$45,64\rightarrow 158$, superposition]\\*[-2ex]
\[\begin{VampireInference}
\begin{VampirePremise}%
~~\mathit{p} (\mathit{s} (\mathit{s} (\mathit{add} (x_{1},x_{1}))),\mathit{s} (x_{1}))
\end{VampirePremise}
\VPremiseSeparator
\begin{VampirePremise}%
~~\sigma_{1}(a0) = \mathit{s} (\mathit{add} (\sigma_{2}(a0),\sigma_{2}(a0))) \Vor \sigma_{1}(a0) = \mathit{add} (\sigma_{2}(a0),\sigma_{2}(a0))
\end{VampirePremise}
\VConclusionSeparator
\begin{VampireConclusion}
~~\mathit{p} (\mathit{s} (\sigma_{1}(a0)),\mathit{s} (\sigma_{2}(a0))) \Vor \sigma_{1}(a0) = \mathit{add} (\sigma_{2}(a0),\sigma_{2}(a0))
\end{VampireConclusion}
\end{VampireInference}
\]
[$24,55\rightarrow 64$, resolution]\\*[-2ex]
\[\begin{VampireInference}
\begin{VampirePremise}%
~~\neg \mathit{p} (x_{0},x_{1}) \Vor \mathit{add} (x_{1},x_{1}) = x_{0} \Vor \mathit{s} (\mathit{add} (x_{1},x_{1})) = x_{0}
\end{VampirePremise}
\VPremiseSeparator
\begin{VampirePremise}%
~~\mathit{p} (\sigma_{1}(a0),\sigma_{2}(a0))
\end{VampirePremise}
\VConclusionSeparator
\begin{VampireConclusion}
~~\sigma_{1}(a0) = \mathit{s} (\mathit{add} (\sigma_{2}(a0),\sigma_{2}(a0))) \Vor \sigma_{1}(a0) = \mathit{add} (\sigma_{2}(a0),\sigma_{2}(a0))
\end{VampireConclusion}
\end{VampireInference}
\]
[$54,29\rightarrow 55$, resolution]\\*[-2ex]
\[\begin{VampireInference}
\begin{VampirePremise}%
~~\mathit{p} (x_{0},\sigma_{0}(x_{0})) \Vor \mathit{p} (\sigma_{1}(a0),\sigma_{2}(a0))
\end{VampirePremise}
\VPremiseSeparator
\begin{VampirePremise}%
~~\neg \mathit{p} (\sigma_{3}(a0),x_{1})
\end{VampirePremise}
\VConclusionSeparator
\begin{VampireConclusion}
~~\mathit{p} (\sigma_{1}(a0),\sigma_{2}(a0))
\end{VampireConclusion}
\end{VampireInference}
\]
[$27,32\rightarrow 54$, resolution]\\*[-2ex]
\[\begin{VampireInference}
\begin{VampirePremise}%
~~\neg \mathit{p} (\mathit{z},x_{5}) \Vor \mathit{p} (\sigma_{1}(a0),\sigma_{2}(a0)) \Vor \mathit{p} (x_{0},\sigma_{0}(x_{0}))
\end{VampirePremise}
\VPremiseSeparator
\begin{VampirePremise}%
~~\mathit{p} (\mathit{z},\mathit{z})
\end{VampirePremise}
\VConclusionSeparator
\begin{VampireConclusion}
~~\mathit{p} (x_{0},\sigma_{0}(x_{0})) \Vor \mathit{p} (\sigma_{1}(a0),\sigma_{2}(a0))
\end{VampireConclusion}
\end{VampireInference}
\]
[$18\rightarrow 27$, cnf transformation]\\*[-2ex]
\[\begin{VampireInference}
\begin{VampirePremise}%
~~(\forall x_{5} )\neg \mathit{p} (\mathit{z},x_{5}) \Vor (\mathit{p} (\sigma_{1}(a0),\sigma_{2}(a0)) \Vand (\forall x_{3} )\neg \mathit{p} (\mathit{s} (\sigma_{1}(a0)),x_{3})) \Vor (\forall x_{0} )\mathit{p} (x_{0},\sigma_{0}(x_{0}))
\end{VampirePremise}
\VConclusionSeparator
\begin{VampireConclusion}
~~\neg \mathit{p} (\mathit{z},x_{5}) \Vor \mathit{p} (\sigma_{1}(a0),\sigma_{2}(a0)) \Vor \mathit{p} (x_{0},\sigma_{0}(x_{0}))
\end{VampireConclusion}
\end{VampireInference}
\]
[$13\rightarrow 24$, cnf transformation]\\*[-2ex]
\[\begin{VampireInference}
\begin{VampirePremise}%
~~(\forall x_{0} \forall x_{1} )((\neg \mathit{p} (x_{0},x_{1}) \Vor \mathit{add} (x_{1},x_{1}) = x_{0} \Vor \mathit{s} (\mathit{add} (x_{1},x_{1})) = x_{0}) \Vand ((\mathit{add} (x_{1},x_{1}) \neq x_{0} \Vand \mathit{s} (\mathit{add} (x_{1},x_{1})) \neq x_{0}) \Vor \mathit{p} (x_{0},x_{1})))
\end{VampirePremise}
\VConclusionSeparator
\begin{VampireConclusion}
~~\neg \mathit{p} (x_{0},x_{1}) \Vor \mathit{add} (x_{1},x_{1}) = x_{0} \Vor \mathit{s} (\mathit{add} (x_{1},x_{1})) = x_{0}
\end{VampireConclusion}
\end{VampireInference}
\]
[$41,38\rightarrow 45$, forward demodulation]\\*[-2ex]
\[\begin{VampireInference}
\begin{VampirePremise}%
~~\mathit{p} (\mathit{s} (\mathit{add} (x_{1},\mathit{s} (x_{1}))),\mathit{s} (x_{1}))
\end{VampirePremise}
\VPremiseSeparator
\begin{VampirePremise}%
~~\mathit{add} (x_{3},\mathit{s} (x_{2})) = \mathit{s} (\mathit{add} (x_{2},x_{3}))
\end{VampirePremise}
\VConclusionSeparator
\begin{VampireConclusion}
~~\mathit{p} (\mathit{s} (\mathit{s} (\mathit{add} (x_{1},x_{1}))),\mathit{s} (x_{1}))
\end{VampireConclusion}
\end{VampireInference}
\]
[$22,23\rightarrow 38$, superposition]\\*[-2ex]
\[\begin{VampireInference}
\begin{VampirePremise}%
~~\mathit{add} (\mathit{s} (x_{0}),x_{1}) = \mathit{s} (\mathit{add} (x_{0},x_{1}))
\end{VampirePremise}
\VPremiseSeparator
\begin{VampirePremise}%
~~\mathit{add} (x_{0},x_{1}) = \mathit{add} (x_{1},x_{0})
\end{VampirePremise}
\VConclusionSeparator
\begin{VampireConclusion}
~~\mathit{add} (x_{3},\mathit{s} (x_{2})) = \mathit{s} (\mathit{add} (x_{2},x_{3}))
\end{VampireConclusion}
\end{VampireInference}
\]
[$3\rightarrow 23$, cnf transformation]\\*[-2ex]
\[\begin{VampireInference}
\begin{VampirePremise}%
~~(\forall x_{0} \forall x_{1} )\mathit{add} (x_{0},x_{1}) = \mathit{add} (x_{1},x_{0})
\end{VampirePremise}
\VConclusionSeparator
\begin{VampireConclusion}
~~\mathit{add} (x_{0},x_{1}) = \mathit{add} (x_{1},x_{0})
\end{VampireConclusion}
\end{VampireInference}
\]
[$2\rightarrow 22$, cnf transformation]\\*[-2ex]
\[\begin{VampireInference}
\begin{VampirePremise}%
~~(\forall x_{0} \forall x_{1} )\mathit{add} (\mathit{s} (x_{0}),x_{1}) = \mathit{s} (\mathit{add} (x_{0},x_{1}))
\end{VampirePremise}
\VConclusionSeparator
\begin{VampireConclusion}
~~\mathit{add} (\mathit{s} (x_{0}),x_{1}) = \mathit{s} (\mathit{add} (x_{0},x_{1}))
\end{VampireConclusion}
\end{VampireInference}
\]
[$31,22\rightarrow 41$, superposition]\\*[-2ex]
\[\begin{VampireInference}
\begin{VampirePremise}%
~~\mathit{p} (\mathit{add} (x_{1},x_{1}),x_{1})
\end{VampirePremise}
\VPremiseSeparator
\begin{VampirePremise}%
~~\mathit{add} (\mathit{s} (x_{0}),x_{1}) = \mathit{s} (\mathit{add} (x_{0},x_{1}))
\end{VampirePremise}
\VConclusionSeparator
\begin{VampireConclusion}
~~\mathit{p} (\mathit{s} (\mathit{add} (x_{1},\mathit{s} (x_{1}))),\mathit{s} (x_{1}))
\end{VampireConclusion}
\end{VampireInference}
\]
[$26\rightarrow 30$, equality resolution]\\*[-2ex]
\[\begin{VampireInference}
\begin{VampirePremise}%
~~\mathit{p} (x_{0},x_{1}) \Vor \mathit{s} (\mathit{add} (x_{1},x_{1})) \neq x_{0}
\end{VampirePremise}
\VConclusionSeparator
\begin{VampireConclusion}
~~\mathit{p} (\mathit{s} (\mathit{add} (x_{1},x_{1})),x_{1})
\end{VampireConclusion}
\end{VampireInference}
\]
[$13\rightarrow 26$, cnf transformation]\\*[-2ex]
\[\begin{VampireInference}
\begin{VampirePremise}%
~~(\forall x_{0} \forall x_{1} )((\neg \mathit{p} (x_{0},x_{1}) \Vor \mathit{add} (x_{1},x_{1}) = x_{0} \Vor \mathit{s} (\mathit{add} (x_{1},x_{1})) = x_{0}) \Vand ((\mathit{add} (x_{1},x_{1}) \neq x_{0} \Vand \mathit{s} (\mathit{add} (x_{1},x_{1})) \neq x_{0}) \Vor \mathit{p} (x_{0},x_{1})))
\end{VampirePremise}
\VConclusionSeparator
\begin{VampireConclusion}
~~\mathit{p} (x_{0},x_{1}) \Vor \mathit{s} (\mathit{add} (x_{1},x_{1})) \neq x_{0}
\end{VampireConclusion}
\end{VampireInference}
\]
[$2$, input]\\*[-2ex]
\[\begin{VampireInference}
\begin{VampireConclusion}
~~(\forall x_{0} \forall x_{1} )\mathit{add} (\mathit{s} (x_{0}),x_{1}) = \mathit{s} (\mathit{add} (x_{0},x_{1}))
\end{VampireConclusion}
\end{VampireInference}
\]
[$3$, input]\\*[-2ex]
\[\begin{VampireInference}
\begin{VampireConclusion}
~~(\forall x_{0} \forall x_{1} )\mathit{add} (x_{0},x_{1}) = \mathit{add} (x_{1},x_{0})
\end{VampireConclusion}
\end{VampireInference}
\]
[$14,17,16,15\rightarrow 18$, skolemisation]\\*[-2ex]
\[\begin{VampireInference}
\begin{VampirePremise}%
~~(\forall x_{5} )\neg \mathit{p} (\mathit{z},x_{5}) \Vor (\exists x_{2} )((\exists x_{4} )\mathit{p} (x_{2},x_{4}) \Vand (\forall x_{3} )\neg \mathit{p} (\mathit{s} (x_{2}),x_{3})) \Vor (\forall x_{0} )(\exists x_{1} )\mathit{p} (x_{0},x_{1})
\end{VampirePremise}
\VPremiseSeparator
\begin{VampirePremise}%
~~(\exists x_{4} )\mathit{p} (\sigma_{1}(a0),x_{4}) \Vimp \mathit{p} (\sigma_{1}(a0),\sigma_{2}(a0))
\end{VampirePremise}
\VPremiseSeparator
\begin{VampirePremise}%
~~(\exists x_{2} )((\exists x_{4} )\mathit{p} (x_{2},x_{4}) \Vand (\forall x_{3} )\neg \mathit{p} (\mathit{s} (x_{2}),x_{3})) \Vimp ((\exists x_{4} )\mathit{p} (\sigma_{1}(a0),x_{4}) \Vand (\forall x_{3} )\neg \mathit{p} (\mathit{s} (\sigma_{1}(a0)),x_{3}))
\end{VampirePremise}
\VPremiseSeparator
\begin{VampirePremise}%
~~(\forall x_{0} )((\exists x_{1} )\mathit{p} (x_{0},x_{1}) \Vimp \mathit{p} (x_{0},\sigma_{0}(x_{0})))
\end{VampirePremise}
\VConclusionSeparator
\begin{VampireConclusion}
~~(\forall x_{5} )\neg \mathit{p} (\mathit{z},x_{5}) \Vor (\mathit{p} (\sigma_{1}(a0),\sigma_{2}(a0)) \Vand (\forall x_{3} )\neg \mathit{p} (\mathit{s} (\sigma_{1}(a0)),x_{3})) \Vor (\forall x_{0} )\mathit{p} (x_{0},\sigma_{0}(x_{0}))
\end{VampireConclusion}
\end{VampireInference}
\]
[$15$, choice axiom]\\*[-2ex]
\[\begin{VampireInference}
\begin{VampireConclusion}
~~(\forall x_{0} )((\exists x_{1} )\mathit{p} (x_{0},x_{1}) \Vimp \mathit{p} (x_{0},\sigma_{0}(x_{0})))
\end{VampireConclusion}
\end{VampireInference}
\]
[$16$, choice axiom]\\*[-2ex]
\[\begin{VampireInference}
\begin{VampireConclusion}
~~(\exists x_{2} )((\exists x_{4} )\mathit{p} (x_{2},x_{4}) \Vand (\forall x_{3} )\neg \mathit{p} (\mathit{s} (x_{2}),x_{3})) \Vimp ((\exists x_{4} )\mathit{p} (\sigma_{1}(a0),x_{4}) \Vand (\forall x_{3} )\neg \mathit{p} (\mathit{s} (\sigma_{1}(a0)),x_{3}))
\end{VampireConclusion}
\end{VampireInference}
\]
[$17$, choice axiom]\\*[-2ex]
\[\begin{VampireInference}
\begin{VampireConclusion}
~~(\exists x_{4} )\mathit{p} (\sigma_{1}(a0),x_{4}) \Vimp \mathit{p} (\sigma_{1}(a0),\sigma_{2}(a0))
\end{VampireConclusion}
\end{VampireInference}
\]
[$10\rightarrow 14$, rectify]\\*[-2ex]
\[\begin{VampireInference}
\begin{VampirePremise}%
~~(\forall x_{3} )\neg \mathit{p} (\mathit{z},x_{3}) \Vor (\exists x_{0} )((\exists x_{1} )\mathit{p} (x_{0},x_{1}) \Vand (\forall x_{2} )\neg \mathit{p} (\mathit{s} (x_{0}),x_{2})) \Vor (\forall x_{4} )(\exists x_{5} )\mathit{p} (x_{4},x_{5})
\end{VampirePremise}
\VConclusionSeparator
\begin{VampireConclusion}
~~(\forall x_{5} )\neg \mathit{p} (\mathit{z},x_{5}) \Vor (\exists x_{2} )((\exists x_{4} )\mathit{p} (x_{2},x_{4}) \Vand (\forall x_{3} )\neg \mathit{p} (\mathit{s} (x_{2}),x_{3})) \Vor (\forall x_{0} )(\exists x_{1} )\mathit{p} (x_{0},x_{1})
\end{VampireConclusion}
\end{VampireInference}
\]
[$9\rightarrow 10$, flattening]\\*[-2ex]
\[\begin{VampireInference}
\begin{VampirePremise}%
~~((\forall x_{3} )\neg \mathit{p} (\mathit{z},x_{3}) \Vor (\exists x_{0} )((\exists x_{1} )\mathit{p} (x_{0},x_{1}) \Vand (\forall x_{2} )\neg \mathit{p} (\mathit{s} (x_{0}),x_{2}))) \Vor (\forall x_{4} )(\exists x_{5} )\mathit{p} (x_{4},x_{5})
\end{VampirePremise}
\VConclusionSeparator
\begin{VampireConclusion}
~~(\forall x_{3} )\neg \mathit{p} (\mathit{z},x_{3}) \Vor (\exists x_{0} )((\exists x_{1} )\mathit{p} (x_{0},x_{1}) \Vand (\forall x_{2} )\neg \mathit{p} (\mathit{s} (x_{0}),x_{2})) \Vor (\forall x_{4} )(\exists x_{5} )\mathit{p} (x_{4},x_{5})
\end{VampireConclusion}
\end{VampireInference}
\]
[$8\rightarrow 9$, ennf transformation]\\*[-2ex]
\[\begin{VampireInference}
\begin{VampirePremise}%
~~((\exists x_{3} )\mathit{p} (\mathit{z},x_{3}) \Vand (\forall x_{0} )((\exists x_{1} )\mathit{p} (x_{0},x_{1}) \Vimp (\exists x_{2} )\mathit{p} (\mathit{s} (x_{0}),x_{2}))) \Vimp (\forall x_{4} )(\exists x_{5} )\mathit{p} (x_{4},x_{5})
\end{VampirePremise}
\VConclusionSeparator
\begin{VampireConclusion}
~~((\forall x_{3} )\neg \mathit{p} (\mathit{z},x_{3}) \Vor (\exists x_{0} )((\exists x_{1} )\mathit{p} (x_{0},x_{1}) \Vand (\forall x_{2} )\neg \mathit{p} (\mathit{s} (x_{0}),x_{2}))) \Vor (\forall x_{4} )(\exists x_{5} )\mathit{p} (x_{4},x_{5})
\end{VampireConclusion}
\end{VampireInference}
\]
[$5\rightarrow 8$, rectify]\\*[-2ex]
\[\begin{VampireInference}
\begin{VampirePremise}%
~~((\exists x_{1} )\mathit{p} (\mathit{z},x_{1}) \Vand (\forall x_{0} )((\exists x_{1} )\mathit{p} (x_{0},x_{1}) \Vimp (\exists x_{1} )\mathit{p} (\mathit{s} (x_{0}),x_{1}))) \Vimp (\forall x_{0} )(\exists x_{1} )\mathit{p} (x_{0},x_{1})
\end{VampirePremise}
\VConclusionSeparator
\begin{VampireConclusion}
~~((\exists x_{3} )\mathit{p} (\mathit{z},x_{3}) \Vand (\forall x_{0} )((\exists x_{1} )\mathit{p} (x_{0},x_{1}) \Vimp (\exists x_{2} )\mathit{p} (\mathit{s} (x_{0}),x_{2}))) \Vimp (\forall x_{4} )(\exists x_{5} )\mathit{p} (x_{4},x_{5})
\end{VampireConclusion}
\end{VampireInference}
\]
[$5$, input]\\*[-2ex]
\[\begin{VampireInference}
\begin{VampireConclusion}
~~((\exists x_{1} )\mathit{p} (\mathit{z},x_{1}) \Vand (\forall x_{0} )((\exists x_{1} )\mathit{p} (x_{0},x_{1}) \Vimp (\exists x_{1} )\mathit{p} (\mathit{s} (x_{0}),x_{1}))) \Vimp (\forall x_{0} )(\exists x_{1} )\mathit{p} (x_{0},x_{1})
\end{VampireConclusion}
\end{VampireInference}
\]
[$12\rightarrow 13$, flattening]\\*[-2ex]
\[\begin{VampireInference}
\begin{VampirePremise}%
~~(\forall x_{0} \forall x_{1} )((\neg \mathit{p} (x_{0},x_{1}) \Vor (\mathit{add} (x_{1},x_{1}) = x_{0} \Vor \mathit{s} (\mathit{add} (x_{1},x_{1})) = x_{0})) \Vand ((\mathit{add} (x_{1},x_{1}) \neq x_{0} \Vand \mathit{s} (\mathit{add} (x_{1},x_{1})) \neq x_{0}) \Vor \mathit{p} (x_{0},x_{1})))
\end{VampirePremise}
\VConclusionSeparator
\begin{VampireConclusion}
~~(\forall x_{0} \forall x_{1} )((\neg \mathit{p} (x_{0},x_{1}) \Vor \mathit{add} (x_{1},x_{1}) = x_{0} \Vor \mathit{s} (\mathit{add} (x_{1},x_{1})) = x_{0}) \Vand ((\mathit{add} (x_{1},x_{1}) \neq x_{0} \Vand \mathit{s} (\mathit{add} (x_{1},x_{1})) \neq x_{0}) \Vor \mathit{p} (x_{0},x_{1})))
\end{VampireConclusion}
\end{VampireInference}
\]
[$4\rightarrow 12$, nnf transformation]\\*[-2ex]
\[\begin{VampireInference}
\begin{VampirePremise}%
~~(\forall x_{0} \forall x_{1} )(\mathit{p} (x_{0},x_{1}) \Viff (\mathit{add} (x_{1},x_{1}) = x_{0} \Vor \mathit{s} (\mathit{add} (x_{1},x_{1})) = x_{0}))
\end{VampirePremise}
\VConclusionSeparator
\begin{VampireConclusion}
~~(\forall x_{0} \forall x_{1} )((\neg \mathit{p} (x_{0},x_{1}) \Vor (\mathit{add} (x_{1},x_{1}) = x_{0} \Vor \mathit{s} (\mathit{add} (x_{1},x_{1})) = x_{0})) \Vand ((\mathit{add} (x_{1},x_{1}) \neq x_{0} \Vand \mathit{s} (\mathit{add} (x_{1},x_{1})) \neq x_{0}) \Vor \mathit{p} (x_{0},x_{1})))
\end{VampireConclusion}
\end{VampireInference}
\]
[$4$, input]\\*[-2ex]
\[\begin{VampireInference}
\begin{VampireConclusion}
~~(\forall x_{0} \forall x_{1} )(\mathit{p} (x_{0},x_{1}) \Viff (\mathit{add} (x_{1},x_{1}) = x_{0} \Vor \mathit{s} (\mathit{add} (x_{1},x_{1})) = x_{0}))
\end{VampireConclusion}
\end{VampireInference}
\]
[$1$, input]\\*[-2ex]
\[\begin{VampireInference}
\begin{VampireConclusion}
~~(\forall x_{0} )\mathit{add} (\mathit{z},x_{0}) = x_{0}
\end{VampireConclusion}
\end{VampireInference}
\]
[$11,19\rightarrow 20$, skolemisation]\\*[-2ex]
\[\begin{VampireInference}
\begin{VampirePremise}%
~~(\exists x_{0} )(\forall x_{1} )\neg \mathit{p} (x_{0},x_{1})
\end{VampirePremise}
\VPremiseSeparator
\begin{VampirePremise}%
~~(\exists x_{0} )(\forall x_{1} )\neg \mathit{p} (x_{0},x_{1}) \Vimp (\forall x_{1} )\neg \mathit{p} (\sigma_{3}(a0),x_{1})
\end{VampirePremise}
\VConclusionSeparator
\begin{VampireConclusion}
~~(\forall x_{1} )\neg \mathit{p} (\sigma_{3}(a0),x_{1})
\end{VampireConclusion}
\end{VampireInference}
\]
[$19$, choice axiom]\\*[-2ex]
\[\begin{VampireInference}
\begin{VampireConclusion}
~~(\exists x_{0} )(\forall x_{1} )\neg \mathit{p} (x_{0},x_{1}) \Vimp (\forall x_{1} )\neg \mathit{p} (\sigma_{3}(a0),x_{1})
\end{VampireConclusion}
\end{VampireInference}
\]
[$7\rightarrow 11$, ennf transformation]\\*[-2ex]
\[\begin{VampireInference}
\begin{VampirePremise}%
~~\neg (\forall x_{0} )(\exists x_{1} )\mathit{p} (x_{0},x_{1})
\end{VampirePremise}
\VConclusionSeparator
\begin{VampireConclusion}
~~(\exists x_{0} )(\forall x_{1} )\neg \mathit{p} (x_{0},x_{1})
\end{VampireConclusion}
\end{VampireInference}
\]
[$6\rightarrow 7$, negated conjecture]\\*[-2ex]
\[\begin{VampireInference}
\begin{VampirePremise}%
~~(\forall x_{0} )(\exists x_{1} )\mathit{p} (x_{0},x_{1})
\end{VampirePremise}
\VConclusionSeparator
\begin{VampireConclusion}
~~\neg (\forall x_{0} )(\exists x_{1} )\mathit{p} (x_{0},x_{1})
\end{VampireConclusion}
\end{VampireInference}
\]
[$6$, input]\\*[-2ex]
\[\begin{VampireInference}
\begin{VampireConclusion}
~~(\forall x_{0} )(\exists x_{1} )\mathit{p} (x_{0},x_{1})
\end{VampireConclusion}
\end{VampireInference}
\]
\end{VampireProof}
\end{document}
